Trestle/Solver/Impl/ApproxMCCommand.lean
@@ -28,7 +28,7 @@ def ApproxMCCommand
   for sampleSet in sampleSet do
     stdin.putStrLn <| "c ind " ++
       (sampleSet.map Dimacs.formatVar ++ ["0"] |> String.intercalate " ")
-  Dimacs.printFormula (stdin.putStr) fml
+  Dimacs.printICnf (stdin.putStr) fml
   stdin.flush
   let output ← IO.asTask child.stdout.readToEnd Task.Priority.dedicated
   match ←child.wait with
