Trestle/Solver/Impl/UniGenCommand.lean
@@ -28,7 +28,7 @@ def UniGenCommand
   let (stdin, child) ← child.takeStdin
   for sampleSet in sampleSet do
     stdin.putStrLn (["c", "ind"] ++ sampleSet.map Dimacs.formatVar ++ ["0"] |> String.intercalate " ")
-  Dimacs.printFormula (stdin.putStr) fml
+  Dimacs.printICnf (stdin.putStr) fml
   stdin.flush
   let output ← IO.asTask child.stdout.readToEnd Task.Priority.dedicated
   let _ ← child.wait
